{
 "cells": [
  {
   "cell_type": "code",
   "execution_count": 1,
   "metadata": {},
   "outputs": [],
   "source": [
    "# Split into the two cases\n",
    "\n",
    "# CASE 1: b=n, a+c=0\n",
    "\n",
    "# Define a polynomial ring. Note all variables are integral.\n",
    "R.<p, ln, lc, A, B, C, delta> = PolynomialRing(Rationals())\n",
    "QuatAlg.<i,j,k> = QuaternionAlgebra(-1, -p)\n",
    "\n",
    "# Basis of order using variables above, i.e. replacing \\ell^b with \\ell^n, and \\ell^a with 1/\\ell^c\n",
    "e0 = (1/2) + (1/(2*lc))*j + ((C + delta*ln*lc)/(2*lc))*k\n",
    "e1 = (lc/(2*ln))*i + (A/ln)*j + (B/(2*ln))*k\n",
    "e2 = (1/lc)*j + (C/lc)*k\n",
    "e3 = ln*k\n",
    "\n",
    "# These are integral by earlier results\n",
    "lambda1 = (2*A + B*C + B*delta*ln*lc)/(2*ln*lc)\n",
    "lambda2 = (p*B^2 + lc^2 + 4*p*A^2)/(4*ln^2)\n",
    "lambda3 = (C^2 + 1 - (delta + 1)*lc^2)/(4*lc^2)\n",
    "lambda4 = (((B - 2*A*C) / (lc^2)) - 1)/2\n",
    "lambda5 = delta*(delta - 1)/4\n",
    "lambda6 = (ln/lc - 1)/2\n",
    "lambda7 = (ln + 1)/2\n",
    "omega1 = (p + 1)/4\n",
    "omega2 = (B + 1)/2\n",
    "omega3 = (delta + C)/2\n",
    "\n",
    "# We show the order is closed under multiplication as each es * et is an integral linear combinations of et so lie in the order\n",
    "# Coefficients consist of addition and multiplication of the integer values above (and integral constants) so are all integral\n",
    "assert(e0*e0 == -(p*(2*lambda6 + 1)*C*delta + 2*p*lambda3 + p*(ln^2*2*lambda5 + (2*lambda7^2 - 2*lambda7 + 1)*delta) + 2*omega1 - 1)*e0 + (p*lambda3 + p*lambda6*C*delta + omega1 + p*delta^2*lambda7*(lambda7 - 1) + p*delta*omega3 - p*lambda5)*e2 + ((2*lambda6 + 1)^2*lambda2*delta + p*delta*((1 - B^2)*lambda3 - (omega2^2 - omega2)*(delta + 1 + 2*(2*lambda6 + 1)*delta*C + delta^2*ln^2) + (2*lambda6 + 1)*lambda1*(B*(2*omega3 - C)*(2*lambda7*(-lc*lambda6 + lambda7 - 1) + lambda7 - (-lc*lambda6 + lambda7 - 1)) - B*omega3 + B*C - A)))*e3)\n",
    "assert(e0*e1 == -p*lambda1*e0 + (-p*(2*lambda6 + 1)*A*delta + p*lambda4 + 2*omega1)*e1 + ((2*lambda6 + 1)*lambda2*(C + ln*lc*delta) - p*(omega2 - 1)*lambda1)*e2 + (-lambda2*((2*lambda6 + 1)*C*delta + (4*lambda3 + delta + 1)) + p*lambda1^2 + p*delta*lambda1*(1 - omega2))*e3)\n",
    "assert(e0*e2 == -p*((2*lambda6 + 1)*C*delta + (4*lambda3 + delta + 1))*e0 - p*(2*lambda6 + 1)^2*delta*e1 + (2*p*lambda3 + 2*omega1 + p*lambda6*delta*(2*ln*lc*lambda1 - B*delta*ln*lc - B*C + C) + p*delta*ln*lc*lambda1 - p*delta*B*delta*(2*lambda7*(-lc*lambda6 + lambda7 - 1) + lambda7 - (-lc*lambda6 + lambda7 - 1)) + p*delta*(B*omega3 - B*C) + p*(omega3*delta - 2*lambda5))*e2 + p*delta*(lambda6*C*delta + lambda4 + 2*lambda3 + omega3*delta - 2*lambda5 + 1)*e3)\n",
    "assert(e0*e3 == -p*(ln^2*delta + (2*lambda6 + 1)*C)*e0 + p*(2*lambda6 + 1)^2*e1 + p*(2*lambda6 + 1)*(delta*(2*lambda7*(-lc*lambda6 + lambda7 - 1) + lambda7 - (-lc*lambda6 + lambda7 - 1)) - omega3 + C - A)*e2 + (2*(2*lambda6 + 1)^2*lambda2 - p*lambda4 + 2*p*lc^2*lambda4*(lambda4 + 1) - 2*p*lc^2*lambda4*(lambda4 + 1) - 2*p*ln^2*lambda1*(lambda1 - B*delta)+ 2*p*B^2*lambda3 - 2*p*B*lambda4 - B*p - 2*p*B^2*ln^2*lambda5 + 2*p*ln^2*lambda5 + p*lambda6*C*delta + 2*p*omega2^2 - 2*p*omega2 + p*delta*omega3 - p*2*lambda5 - p*delta*(ln^2 - 1)*(2*omega2^2 - 2*omega2))*e3)\n",
    "assert(e1*e0 == -p*lambda1*e0 + (-p*lambda4 + p*(2*lambda6 + 1)*A*delta - 2*omega1 + 1)*e1 + (-(2*lambda6 + 1)*lambda2*(ln*lc*delta + C) + p*lambda1*omega2)*e2 + (lambda2*((2*lambda6 + 1)*C*delta + (4*lambda3 + delta + 1)) - p*lambda1^2 + p*omega2*delta*lambda1)*e3)\n",
    "assert(e1*e1 == -2*lambda2*e0 + lambda2*e2 + delta*lambda2*e3)\n",
    "assert(e1*e2 == -p*(2*lambda1 - B*delta)*e0 - p*(2*lambda4 + 1)*e1 + (p*lambda1 + p*B*lambda1 - p*B*delta*omega2 - 2*(2*lambda6 + 1)*lambda2*C)*e2 + (2*lambda2*(4*lambda3 + delta + 1) - p*(2*lambda1 - B*delta)*(lambda1 - omega2*delta))*e3)\n",
    "assert(e1*e3 == -p*B*e0 + 2*p*(2*lambda6 + 1)*A*e1 + (-2*ln^2*lambda2 + p*B*omega2)*e2 + (2*(2*lambda6 + 1)*lambda2*C + p*(-lambda1*B + delta*omega2*B))*e3)\n",
    "assert(e2*e0 == -p*((2*lambda6 + 1)*C*delta + (4*lambda3 + delta + 1))*e0 + p*(2*lambda6 + 1)^2*delta*e1 + (-p*(2*lambda6 + 1)*A*delta + p*lambda6*C*delta + 2*p*lambda3 + p*(omega3*delta - 2*lambda5) + 2*omega1)*e2 + p*delta*(lambda6*C*delta - lambda4 + omega3*delta - 2*lambda5 + 2*lambda3)*e3)\n",
    "assert(e2*e1 == -p*(2*lambda1 - B*delta)*e0 + p*(2*lambda4 + 1)*e1 + (2*(2*lambda6 + 1)*lambda2*C - p*(omega2 - 1)*(2*lambda1 - B*delta))*e2 + (-2*lambda2*(4*lambda3 + delta + 1) + p*(delta^2*B*(omega2 - 1) - (2*B - 1)*delta*lambda1 + 2*lambda1^2))*e3)\n",
    "assert(e2*e2 == -2*p*(4*lambda3 + delta + 1)*e0 + p*(4*lambda3 + delta + 1)*e2 + p*delta*(4*lambda3 + delta + 1)*e3)\n",
    "assert(e2*e3 == -2*p*(2*lambda6 + 1)*C*e0 + 2*p*(2*lambda6 + 1)^2*e1 + p*(2*lambda6 + 1)*(-2*A + C)*e2 + (p*(2*lambda6 + 1)*C*delta - p*(2*lambda4 + 1))*e3)\n",
    "assert(e3*e0 == (-p*ln^2*delta - p*(2*lambda6 + 1)*C)*e0 - p*(2*lambda6 + 1)^2*e1 + p*(2*lambda6 + 1)*(-(C+ln*lc*delta)*(omega2 - 1) + ln*lc*lambda1)*e2 + (lambda4*p + 2*(2*lambda6 + 1)^2*lambda2 + 2*p*A^2*(4*lambda3 + delta + 1) - 2*p*lc^2*lambda4*(lambda4+1) - 2*p*A*(2*lambda1 - B*delta)*(2*lambda6 + 1) - 2*p*(-lc*lambda6 + lambda7 - 1)*((-lc*lambda6 + lambda7 - 1) + 1) + p*(2*lambda6 + 1)*delta*((2*omega3 - C)*(2*lambda7*(-lc*lambda6 + lambda7 - 1) + lambda7 - (-lc*lambda6 + lambda7 - 1)) - omega3 + C))*e3)\n",
    "assert(e3*e1 == -p*B*e0 + -2*p*(2*lambda6 + 1)*A*e1 + (2*ln^2*lambda2 - p*B*(omega2 - 1))*e2 + (p*lambda1*B - (omega2 - 1)*p*delta*B - 2*(2*lambda6 + 1)*lambda2*C)*e3)\n",
    "assert(e3*e2 == -2*p*(2*lambda6 + 1)*C*e0 - 2*p*(2*lambda6 + 1)^2*e1 + p*(2*lambda6 + 1)*(2*A + C)*e2 + p*((2*lambda6 + 1)*C*delta + (2*lambda4 + 1))*e3)\n",
    "assert(e3*e3 == -2*p*ln^2*e0 + p*ln^2*e2 + p*ln^2*delta*e3)\n",
    "\n",
    "\n",
    "\n",
    "# CASE 2: a+b=n, c=0, a>=0\n",
    "\n",
    "# Define a polynomial ring. Note all variables are integral.\n",
    "R.<p, ln, lb, A, B, C, delta> = PolynomialRing(Rationals())\n",
    "QuatAlg.<i,j,k> = QuaternionAlgebra(-1, -p)\n",
    "\n",
    "# Basis of order using variables above, i.e. replacing \\ell^a with \\ell^n/\\ell^b, and \\ell^c with 1\n",
    "e0 = (1/2) + (ln/(2*lb))*j + ((C + delta*lb)/(2))*k\n",
    "e1 = (1/(2*ln))*i + (A/ln)*j + (B/(2*lb))*k\n",
    "e2 = (ln/lb)*j + (C)*k\n",
    "e3 = lb*k\n",
    "\n",
    "# These are integral by earlier results\n",
    "mu1 = (2*A + B*C + B*delta*lb)/(2*lb)\n",
    "mu2 = (p*ln^2*B^2 + lb^2 + 4*p*A^2*lb^2)/(4*ln^2*lb^2)\n",
    "mu3 = (ln/lb - 1)/2\n",
    "mu4 = (lb + 1)/2\n",
    "omega1 = (p + 1)/4\n",
    "omega2 = (B + 1)/2\n",
    "omega3 = (delta + C)/2\n",
    "\n",
    "# We show the order is closed under multiplication as each es * et is an integral linear combinations of et so lie in the order\n",
    "# Coefficients consist of addition and multiplication of the integer values above (and integral constants) so are all integral\n",
    "assert(e0*e0 == (-p*lb*C*delta - 2*p*(mu3^2 + mu3) - p*(2*(delta*mu4 + omega3 - delta)^2 - lb*C*delta) - 2*omega1 + 1)*e0 + (p*(delta*mu4 + omega3 - delta)^2 + p*mu3*(mu3+1) + omega1)*e2 + delta*(p*(delta*mu4 + omega3 - delta)^2 + p*mu3*(mu3+1) + omega1)*e3)\n",
    "assert(e0*e1 == -p*mu1*e0 + (-p*lb*A*delta - p*A*C + 2*p*mu3*(mu3 + 1)*B + 4*omega2*omega1 - 2*omega1 - omega2 + 1)*e1 + (lb*mu2*C + delta*(lb^2*mu2 - p*omega2*(omega2 - 1)) + p*(omega2 - 1)*delta*omega2 - p*(omega2 - 1)*mu1)*e2 + (-mu2*((2*mu3+1)^2 + C^2 + lb*C*delta) + p*mu1^2 - p*delta*mu1*(omega2 - 1))*e3)\n",
    "assert(e0*e2 == (-p*lb*C*delta - p*C^2 - p*(2*mu3+1)^2)*e0 - p*ln^2*delta*e1 + (p*lb*A*delta + p*C*(delta*mu4 + omega3 - delta) + 2*p*mu3*(mu3 + 1) + 2*omega1)*e2 + delta*(p*C*(delta*mu4 + omega3 - delta) - p*A*C + 2*p*mu3*(mu3 + 1)*B + p*omega2 + 2*p*mu3*(mu3 + 1))*e3)\n",
    "assert(e0*e3 == (-p*lb^2*delta - p*lb*C)*e0 + p*ln^2*e1 + (p*lb*(delta*mu4 + omega3 - delta) - p*lb*A)*e2 + (p*lb*delta*(delta*mu4 + omega3 - delta) + p*A*C - 2*p*mu3*(mu3 + 1)*B - 4*omega2*omega1 + 2*omega1 + omega2)*e3)\n",
    "assert(e1*e0 == -p*mu1*e0 + (p*lb*A*delta + p*A*C - 2*p*mu3*(mu3 + 1)*B - 4*omega2*omega1 + 2*omega1 + omega2)*e1 + (p*omega2*mu1 - lb*mu2*(C + lb*delta))*e2 + (mu2*((2*mu3+1)^2 + C^2 + lb*C*delta) - p*mu1^2 + p*mu1*omega2*delta)*e3)\n",
    "assert(e1*e1 == -2*mu2*e0 + mu2*e2 + mu2*delta*e3)\n",
    "assert(e1*e2 == -p*(2*mu1 - B*delta)*e0 + (2*p*A*C - p*(2*mu3+1)^2*B)*e1 + (p*mu1*(B+1) - p*B*delta*omega2 - 2*lb*mu2*C)*e2 + (2*mu2*(C^2 + (2*mu3+1)^2) + p*(-2*mu1^2 + delta*(mu1*(1+2*B) + B*delta*(omega2 - 1 - B))))*e3)\n",
    "assert(e1*e3 == -p*B*e0 + 2*p*lb*A*e1 + (-2*lb^2*mu2 + p*B*omega2)*e2 + (2*lb*mu2*C - p*B*(mu1 - omega2*delta))*e3)\n",
    "assert(e2*e0 == (-p*lb*C*delta - p*C^2 - p*(2*mu3+1)^2)*e0 + p*ln^2*delta*e1 + ((-2*p*lb^3*A*delta + p*lb^3*C*delta + p*lb^2*C^2 + p*ln^2 + lb^2)/(2*lb^2))*e2 + p*delta*((2*omega3*mu4 - C*mu4 - omega3 + C)*C + A*C - omega2 + 1 - 2*mu3*B*(mu3 + 1) + 2*mu3^2 + 2*mu3)*e3)\n",
    "assert(e2*e1 == -p*(2*mu1 - B*delta)*e0 + (-2*p*A*C + p*(2*mu3+1)^2*B)*e1 + (2*lb*mu2*C - p*(2*mu1 - B*delta)*(omega2 - 1))*e2 - (2*mu2*(C^2 + (2*mu3+1)^2) + p*(-2*mu1^2 + B*omega2*delta^2 + (2*mu1 - B*delta)*B*delta - delta*mu1))*e3)\n",
    "assert(e2*e2 == 2*(-p*C^2 - p*(2*mu3+1)^2)*e0 + (p*C^2 + p*(2*mu3+1)^2)*e2 + (p*C^2*delta + p*(2*mu3+1)^2*delta)*e3)\n",
    "assert(e2*e3 == -2*p*lb*C*e0 + 2*p*ln^2*e1 + (-2*p*lb*A + p*lb*C)*e2 + (p*lb*C*delta + 2*p*A*C - p*(2*mu3+1)^2*B)*e3)\n",
    "assert(e3*e0 == (-p*lb^2*delta - p*lb*C)*e0 - p*ln^2*e1 + (p*lb*(delta*mu4 + omega3 - delta) + p*lb*A)*e2 + (p*lb*delta*(2*omega3*mu4 - C*mu4 - omega3 + C) - p*A*C + 2*p*(mu3^2 + mu3)*B + 4*omega2*omega1 - 2*omega1 - omega2 + 1)*e3)\n",
    "assert(e3*e1 == -p*B*e0 - 2*p*lb*A*e1 + (2*lb^2*mu2 - p*B*(omega2 - 1))*e2 + (p*B*(mu1 - (omega2 - 1)*delta) - 2*lb*mu2*C)*e3)\n",
    "assert(e3*e2 == -2*p*lb*C*e0 - 2*p*ln^2*e1 + (2*p*lb*A + p*lb*C)*e2 + (p*lb*C*delta - 2*p*A*C + p*(2*mu3+1)^2*B)*e3)\n",
    "assert(e3*e3 == -2*p*lb^2*e0 + p*lb^2*e2 + p*lb^2*delta*e3)"
   ]
  }
 ],
 "metadata": {
  "kernelspec": {
   "display_name": "SageMath 10.3.beta8",
   "language": "sage",
   "name": "sagemath"
  },
  "language_info": {
   "codemirror_mode": {
    "name": "ipython",
    "version": 3
   },
   "file_extension": ".py",
   "mimetype": "text/x-python",
   "name": "python",
   "nbconvert_exporter": "python",
   "pygments_lexer": "ipython3",
   "version": "3.10.6"
  }
 },
 "nbformat": 4,
 "nbformat_minor": 2
}
