{
 "cells": [
  {
   "cell_type": "code",
   "execution_count": 1,
   "metadata": {},
   "outputs": [],
   "source": [
    "# Split into the two cases\n",
    "\n",
    "# CASE 1: b=n, a+c=0\n",
    "\n",
    "# Define a polynomial ring. Note all variables are integral.\n",
    "R.<p, ln, lc, A, B, C, delta> = PolynomialRing(Rationals())\n",
    "QuatAlg.<i,j,k> = QuaternionAlgebra(-1, -p)\n",
    "\n",
    "# Basis of the lattice using variables above, i.e. replacing \\ell^b with \\ell^n, and \\ell^a with 1/\\ell^c\n",
    "e0 = (1/2) - (C/2)*i + ((B - 2*A*C)/(2*lc))*j - ((2*A + B*C)/(2*lc))*k\n",
    "e1 = (lc/2)*i + A*j + (B/2)*k \n",
    "e2 = (ln/lc)*j + C*(ln/lc)*k \n",
    "e3 = ln*k\n",
    "\n",
    "# Basis of O0\n",
    "f0 = (1+j)/2\n",
    "f1 = (i+k)/2\n",
    "f2 = j\n",
    "f3 = k\n",
    "\n",
    "# These are integral by earlier results\n",
    "lambda1 = (2*A + B*C + B*delta*ln*lc)/(2*ln*lc)\n",
    "lambda2 = (p*B^2 + lc^2 + 4*p*A^2)/(4*ln^2)\n",
    "lambda3 = (C^2 + 1 - (delta + 1)*lc^2)/(4*lc^2)\n",
    "lambda4 = (((B - 2*A*C) / (lc^2)) - 1)/2\n",
    "lambda5 = delta*(delta - 1)/4\n",
    "lambda6 = (ln/lc - 1)/2\n",
    "lambda7 = (ln + 1)/2\n",
    "omega1 = (p + 1)/4\n",
    "omega2 = (B + 1)/2\n",
    "omega3 = (delta + C)/2\n",
    "\n",
    "# We show the lattice contained within O0 by writing e_t as an integral linear combination of f_t\n",
    "# Coefficients consist of addition and multiplication of the integer values above (and integral constants) so are all integral\n",
    "assert(e0 == f0 - C*f1 + (lc*lambda4 + -lc*lambda6 + lambda7 - 1)*f2 + (-ln*lambda1 + (2*omega2*lambda7 - omega2 - lambda7)*delta + omega3)*f3)\n",
    "assert(e1 == lc*f1 + A*f2 + (-(-lc*lambda6 + lambda7 - 1) + omega2 - 1)*f3)\n",
    "assert(e2 == (2*lambda6+1)*f2 + (2*lambda6+1)*C*f3)\n",
    "assert(e3 == ln*f3)\n",
    "\n",
    "# We show the lattice is a left ideal as each f_s * e_t is an integral linear combinations of e_t so lie in the order\n",
    "# Coefficients consist of addition and multiplication of the integer values above (and integral constants) so are all integral\n",
    "assert(f0*e0 == (-p*lc*lambda4 - 4*(-lc*lambda6 + lambda7 - 1)*omega1 - 2*omega1 + (-lc*lambda6 + lambda7 - 1) + 1)*e0 - p*(C*(2*lambda4 + 1) + A*(4*lambda3 + delta + 1))*e1 + lambda2*(2*lambda6+1)*e2)\n",
    "assert(f0*e1 == -p*A*e0 + (p*lc*lambda4 + 4*(-lc*lambda6 + lambda7 - 1)*omega1 + 2*omega1 - (-lc*lambda6 + lambda7 - 1))*e1 - lambda2*(2*lambda6+1)*e3)\n",
    "assert(f0*e2 == -p*(2*lambda6+1)*e0 + (p*lc*lambda4 + 4*(-lc*lambda6 + lambda7 - 1)*omega1 + 2*omega1 - (-lc*lambda6 + lambda7 - 1))*e2 - p*(C*(2*lambda4 + 1) + A*(4*lambda3 + delta + 1))*e3)\n",
    "assert(f0*e3 == p*(2*lambda6+1)*e1 - p*A*e2 + (-p*lc*lambda4 - 4*(-lc*lambda6 + lambda7 - 1)*omega1 - 2*omega1 + (-lc*lambda6 + lambda7 - 1) + 1)*e3)\n",
    "assert(f1*e0 == (p*ln*lambda1 + p*((2*omega2*lambda7 - omega2 - lambda7)*delta + omega3) - (2*omega1-1)*C - p*ln*B*delta)*e0 + ((4*omega2*omega1 - omega2 - 2*omega1 - (-lc*lambda6 + lambda7 - 1) + lc)*(4*lambda3 + delta + 1) - p*(2*lambda4 + 1))*e1 - (2*lambda6+1)*lambda2*C*e2 + ln*lambda2*(4*lambda3 + delta + 1)*e3)\n",
    "assert(f1*e1 == -(4*omega2*omega1 - omega2 - 2*omega1 + (-lc*lambda6 + lambda7 - 1) + 1)*e0 - (p*((2*omega2*lambda7 - omega2 - lambda7)*delta + omega3 + ln*lambda1) - (2*omega1-1)*C - p*ln*B*delta)*e1 + ln*lambda2*e2 - lambda2*C*(2*lambda6+1)*e3)\n",
    "assert(f1*e2 == -p*(2*lambda6+1)*C*e0 - p*ln*(4*lambda3 + delta + 1)*e1 + (p*ln*lambda1 - p*((2*omega2*lambda7 - omega2 - lambda7)*delta + omega3) + (2*omega1-1)*C)*e2 + (p*(2*lambda4 + 1) - (4*lambda3 + delta + 1)*(4*omega2*omega1 - omega2 - 2*omega1 - (-lc*lambda6 + lambda7 - 1)))*e3)\n",
    "assert(f1*e3 == -p*ln*e0 - p*(2*lambda6+1)*C*e1 + (4*omega2*omega1 - omega2 - 2*omega1 - (-lc*lambda6 + lambda7 - 1))*e2 + (p*(-ln*lambda1 + (2*omega2*lambda7 - omega2 - lambda7)*delta + omega3) - (2*omega1-1)*C)*e3)\n",
    "assert(f2*e0 == -p*lc*(2*lambda4 + 1)*e0 + 2*p*(A*(4*lambda3 + delta + 1) - (2*lambda1 - B*delta)*(2*lambda6+1))*e1 + 2*(2*lambda6+1)*lambda2*e2)\n",
    "assert(f2*e1 == -2*p*A*e0 + p*lc*(2*lambda4 + 1)*e1 - 2*(2*lambda6+1)*lambda2*e3)\n",
    "assert(f2*e2 == -2*p*(2*lambda6+1)*e0 + p*lc*(2*lambda4 + 1)*e2 + 2*p*(A*(4*lambda3 + delta + 1) - (2*lambda1 - B*delta)*(2*lambda6+1))*e3)\n",
    "assert(f2*e3 == 2*p*(2*lambda6+1)*e1 - 2*p*A*e2 - p*lc*(2*lambda4 + 1)*e3)\n",
    "assert(f3*e0 == p*ln*(2*lambda1 - B*delta)*e0 + p*(B*(4*lambda3 + delta + 1) - 2*(2*lambda4 + 1))*e1 - 2*lambda2*(2*lambda6+1)*C*e2 + 2*ln*lambda2*(4*lambda3 + delta + 1)*e3)\n",
    "assert(f3*e1 == -p*B*e0 - p*ln*(2*lambda1 - B*delta)*e1 + 2*ln*lambda2*e2 - 2*lambda2*C*(2*lambda6+1)*e3)\n",
    "assert(f3*e2 == -2*p*(2*lambda6+1)*C*e0 - 2*p*ln*(4*lambda3 + delta + 1)*e1 + p*(2*lambda1 - B*delta)*ln*e2 + p*(-B*(4*lambda3 + delta + 1) + 2*(2*lambda4 + 1))*e3)\n",
    "assert(f3*e3 == -2*p*ln*e0 - 2*p*(2*lambda6+1)*C*e1 + p*B*e2 - p*ln*(2*lambda1 - B*delta)*e3)\n",
    "\n",
    "\n",
    "\n",
    "# CASE 2: a+b=n, c=0, a>=0\n",
    "\n",
    "# Define a polynomial ring. Note all variables are integral.\n",
    "R.<p, ln, lb, A, B, C, delta> = PolynomialRing(Rationals())\n",
    "QuatAlg.<i,j,k> = QuaternionAlgebra(-1, -p)\n",
    "\n",
    "# Basis of the lattice using variables above, i.e. replacing \\ell^a with \\ell^n/\\ell^b, and \\ell^c with 1\n",
    "e0 = (1/2) - (C/2)*i + ((B*ln - 2*lb*A*C)/(2*lb))*j - ((2*A*lb + B*C*ln)/(2*lb))*k\n",
    "e1 = (1/2)*i + A*j + ((B*ln)/(2*lb))*k \n",
    "e2 = ln*j\n",
    "e3 = ln*k\n",
    "\n",
    "# Basis of O0\n",
    "f0 = (1+j)/2\n",
    "f1 = (i+k)/2\n",
    "f2 = j\n",
    "f3 = k\n",
    "\n",
    "# These are integral by earlier results\n",
    "mu1 = (2*A + B*C + B*delta*lb)/(2*lb)\n",
    "mu2 = (p*ln^2*B^2 + lb^2 + 4*p*A^2*lb^2)/(4*ln^2*lb^2)\n",
    "mu3 = (ln/lb - 1)/2\n",
    "mu4 = (lb + 1)/2\n",
    "omega1 = (p + 1)/4\n",
    "omega2 = (B + 1)/2\n",
    "omega3 = (delta + C)/2\n",
    "\n",
    "# We show the lattice contained within O0 by writing e_t as an integral linear combination of f_t\n",
    "# Coefficients consist of addition and multiplication of the integer values above (and integral constants) so are all integral\n",
    "assert(e0 == f0 - C*f1 + (-A*C - 1 + omega2 + mu3*B)*f2 + (-mu3*B*C - A - C*(omega2 - 1))*f3)\n",
    "assert(e1 == f1 + A*f2 + (mu3*B + omega2 - 1)*f3)\n",
    "assert(e2 == ln*f2)\n",
    "assert(e3 == ln*f3)\n",
    "\n",
    "# We show the lattice is a left ideal as each f_s * e_t is an integral linear combinations of e_t so lie in the order\n",
    "# Coefficients consist of addition and multiplication of the integer values above (and integral constants) so are all integral\n",
    "assert(f0*e0 == (p*A*C - p*mu3*B - 4*omega1*omega2 + 2*omega1 + omega2)*e0 + p*(A*C^2 - (2*mu3+1)*B*C - A)*e1 + ln*mu2*e2 + ln*mu2*C*e3)\n",
    "assert(f0*e1 == -p*A*e0 + (-p*A*C + p*mu3*B + 4*omega1*omega2 - 2*omega1 - omega2 + 1)*e1 - ln*mu2*e3)\n",
    "assert(f0*e2 == -p*ln*e0 - p*ln*C*e1 + (p*mu3*B + 4*omega1*omega2 - 2*omega1 - omega2 + 1)*e2 - p*A*e3)\n",
    "assert(f0*e3 == p*ln*e1 - p*A*e2 + (-p*mu3*B - 4*omega1*omega2 + 2*omega1 + omega2)*e3)\n",
    "assert(f1*e0 == (p*mu3*B*C + p*A + 4*omega1*omega2*C - 2*omega1*C - omega2*C + C)*e0 + (p*mu3*B*C^2 + 2*p*A*C - p*mu3*B + (4*omega1*omega2 - 2*omega1 - omega2 + 1)*(C^2-1) + 1)*e1 - ln*mu2*C*e2 + ln*mu2*e3)\n",
    "assert(f1*e1 == -(p*mu3*B + 4*omega1*omega2 - 2*omega1 - omega2 + 1)*e0 - (p*mu3*B*C + p*A + 4*omega1*omega2*C - 2*omega1*C - omega2*C + C)*e1 + ln*mu2*e2)\n",
    "assert(f1*e2 == -p*ln*e1 + p*A*e2 + (p*mu3*B + 4*omega1*omega2 - 2*omega1 - omega2 + 1)*e3)\n",
    "assert(f1*e3 == -p*ln*e0 - p*ln*C*e1 + (mu3*p*B + 4*omega1*omega2 - 2*omega1 - omega2)*e2 - p*A*e3)\n",
    "assert(f2*e0 == (2*p*A*C - p*(2*mu3+1)*B)*e0 + 2*p*(A*C^2 - (2*mu3+1)*B*C - A)*e1 + 2*ln*mu2*e2 + 2*ln*mu2*C*e3)\n",
    "assert(f2*e1 == -2*p*A*e0 + (-2*p*A*C + p*(2*mu3+1)*B)*e1 - 2*ln*mu2*e3)\n",
    "assert(f2*e2 == -2*p*ln*e0 - 2*p*ln*C*e1 + p*(2*mu3+1)*B*e2 - 2*p*A*e3)\n",
    "assert(f2*e3 == 2*p*ln*e1 - 2*p*A*e2 - p*(2*mu3+1)*B*e3)\n",
    "assert(f3*e0 == (p*(2*mu3+1)*B*C + 2*p*A)*e0 + (p*(2*mu3+1)*B*C^2 + 4*p*A*C - p*(2*mu3+1)*B)*e1 - 2*ln*mu2*C*e2 + 2*ln*mu2*e3)\n",
    "assert(f3*e1 == -p*(2*mu3+1)*B*e0 + (-p*(2*mu3+1)*B*C - 2*p*A)*e1 + 2*ln*mu2*e2)\n",
    "assert(f3*e2 == -2*p*ln*e1 + 2*p*A*e2 + p*(2*mu3+1)*B*e3)\n",
    "assert(f3*e3 == -2*p*ln*e0 - 2*p*ln*C*e1 + p*(2*mu3+1)*B*e2 - 2*p*A*e3)"
   ]
  }
 ],
 "metadata": {
  "kernelspec": {
   "display_name": "SageMath 10.3.beta8",
   "language": "sage",
   "name": "sagemath"
  },
  "language_info": {
   "codemirror_mode": {
    "name": "ipython",
    "version": 3
   },
   "file_extension": ".py",
   "mimetype": "text/x-python",
   "name": "python",
   "nbconvert_exporter": "python",
   "pygments_lexer": "ipython3",
   "version": "3.10.6"
  }
 },
 "nbformat": 4,
 "nbformat_minor": 2
}
