{
 "cells": [
  {
   "cell_type": "code",
   "execution_count": 1,
   "metadata": {},
   "outputs": [],
   "source": [
    "# Split into the two cases\n",
    "\n",
    "# CASE 1: b=n, a+c=0\n",
    "\n",
    "# Define a polynomial ring. Note all variables are integral.\n",
    "R.<p, ln, lc, A, B, C, delta> = PolynomialRing(Rationals())\n",
    "QuatAlg.<i,j,k> = QuaternionAlgebra(-1, -p)\n",
    "\n",
    "# Basis of the lattice using variables above, i.e. replacing \\ell^b with \\ell^n, and \\ell^a with 1/\\ell^c\n",
    "e0 = (1/2) - (C/2)*i + ((B - 2*A*C)/(2*lc))*j - ((2*A + B*C)/(2*lc))*k\n",
    "e1 = (lc/2)*i + A*j + (B/2)*k \n",
    "e2 = (ln/lc)*j + C*(ln/lc)*k \n",
    "e3 = ln*k\n",
    "\n",
    "# Basis of maximal order O\n",
    "g0 = (1/2) + (1/(2*lc))*j + ((C + delta*ln*lc)/(2*lc))*k\n",
    "g1 = (lc/(2*ln))*i + (A/ln)*j + (B/(2*ln))*k\n",
    "g2 = (1/lc)*j + (C/lc)*k\n",
    "g3 = ln*k\n",
    "\n",
    "# These are integral by earlier results\n",
    "lambda1 = (2*A + B*C + B*delta*ln*lc)/(2*ln*lc)\n",
    "lambda2 = (p*B^2 + lc^2 + 4*p*A^2)/(4*ln^2)\n",
    "lambda3 = (C^2 + 1 - (delta + 1)*lc^2)/(4*lc^2)\n",
    "lambda4 = (((B - 2*A*C) / (lc^2)) - 1)/2\n",
    "lambda5 = delta*(delta - 1)/4\n",
    "lambda6 = (ln/lc - 1)/2\n",
    "lambda7 = (ln + 1)/2\n",
    "omega1 = (p + 1)/4\n",
    "omega2 = (B + 1)/2\n",
    "omega3 = (delta + C)/2\n",
    "\n",
    "# We show the lattice contained within O by writing e_t as an integral linear combination of g_t\n",
    "# Coefficients consist of addition and multiplication of the integer values above (and integral constants) so are all integral\n",
    "assert(e0 == g0 - (2*lambda6 + 1)*C*g1 + (omega2-1)*g2 - (lambda1 - (omega2-1)*delta)*g3)\n",
    "assert(e1 == ln*g1)\n",
    "assert(e2 == ln*g2)\n",
    "assert(e3 == g3)\n",
    "\n",
    "# We show the lattice is a right ideal as each e_t * g_s is an integral linear combinations of e_t so lie in the order\n",
    "# Coefficients consist of addition and multiplication of the integer values above (and integral constants) so are all integral\n",
    "assert(e0*g0 == (2*lambda2*(2*lambda6+1)^2 + p*ln^2*lambda1*delta - p*B*(4*2*lambda5*lambda7^2 + 2*lambda7^2*delta - ln*delta^2 - 2*lambda5) - 2*p*B*lambda3 - p*(omega2-1) - 2*omega1 +1 - 2*lambda2*(2*lambda6+1)^2 + p*C*(2*lambda1 - B*delta)*(2*lambda6+1))*e0 + p*ln*(4*lambda3 + delta + 1)*lambda1*e1 + (-p*ln*(2*lambda1 - B*delta)*lambda1 + ln*lambda2*(delta + 1 + (2*lambda6+1)*C*delta) + 4*ln*lambda2*lambda3)*e2 + (lambda2*(-C+ln*lc*delta)*(4*lambda3 + delta + 1)*(2*lambda6+1) - 2*lambda2*C^2*delta*(2*lambda6+1)^2 - p*B*delta*(2*lambda4 + 1) + p*lambda1*B*(4*lambda3 + delta + 1) - p*(2*lambda1 - B*delta)*(2*lambda4 + 1))*e3)\n",
    "assert(e0*g1 == 2*lambda2*C*(2*lambda6+1)*e0 + 2*ln*lambda2*(4*lambda3 + delta + 1)*e1 - ln*lambda2*(2*lambda1 - B*delta)*e2 + lambda2*(-2*(2*lambda4 + 1) + B*(4*lambda3 + delta + 1))*e3)\n",
    "assert(e0*g2 == p*(B*(4*lambda3 + delta + 1) - 2*(2*lambda4 + 1))*e0 + p*(4*lambda3 + delta + 1)*(2*lambda1 - B*delta)*ln*e1 + (-p*ln*(2*lambda1 - B*delta)^2 + 2*ln*lambda2*(4*lambda3 + delta + 1))*e2 + (-2*lambda2*C*(4*lambda3 + delta + 1)*(2*lambda6+1) - p*(2*lambda4 + 1)*(2*lambda1 - B*delta) + p*(2*lambda1 - B*delta)^2*C*(2*lambda6+1))*e3)\n",
    "assert(e0*g3 == p*(B*C + 2*A)*(2*lambda6+1)*e0 + p*ln*B*(4*lambda3 + delta + 1)*e1 + (- p*ln*B*(2*lambda1 - B*delta) + 2*ln*(2*lambda6+1)*lambda2*C)*e2 + (-2*(2*lambda6+1)^2*lambda2*(C^2-1) + p*B*(B*(4*lambda3 + delta + 1) - 2*(2*lambda4 + 1)))*e3)\n",
    "assert(e1*g0 == -p*ln*lambda1*e0 + (-p*ln^2*lambda1*delta + 2*p*(2*lambda6+1)*A*delta - 2*p*B*lambda3 + p*B*(4*2*lambda5*lambda7^2 + 2*lambda7^2*delta - ln*delta^2 - 2*lambda5) - p*B*delta - 4*omega1*omega2 + 2*omega1 + omega2)*e1 + (-ln^2*delta*lambda2 + p*B*lambda1 - (2*lambda6+1)*lambda2*C)*e2 + ln*((2*lambda6+1)*lambda2*C*delta - p*(2*lambda1 - B*delta)*lambda1 + lambda2*(4*lambda3 + delta + 1))*e3)\n",
    "assert(e1*g1 == -2*ln*lambda2*e0 - 2*lambda2*(2*lambda6+1)*C*e1 + lambda2*B*e2 - ln*lambda2*(2*lambda1 - B*delta)*e3)\n",
    "assert(e1*g2 == -p*(2*lambda1 - B*delta)*ln*e0 - p*B*(4*lambda3 + delta + 1)*e1 + ((2*lambda1 - B*delta)*p*B - 2*(2*lambda6+1)*lambda2*C)*e2 + (2*ln*lambda2*(4*lambda3 + delta + 1) - p*lc*(2*lambda1 - B*delta)*(2*lambda4 + 1)*C - 2*p*A*lc*(4*lambda3 + delta + 1)*(2*lambda1 - B*delta))*e3)\n",
    "assert(e1*g3 == -p*ln*B*e0 + p*(2*lambda6+1)*(-B*C + 2*A)*e1 + (-2*ln^2*lambda2 + p*B^2)*e2 + (- p*ln*B*(2*lambda1 - B*delta) + 2*ln*lambda2*(2*lambda6+1)*C)*e3)\n",
    "assert(e2*g0 == -p*ln*(C*delta*(2*lambda6+1) + (4*lambda3 + delta + 1))*e0 + p*(2*lambda6+1)*(-(2*lambda6+1)*C^2*delta - C*(4*lambda3 + delta + 1) + (2*lambda6+1)*delta)*e1 + (p*delta*(-2*A + ln*lc*lambda1)*(2*lambda6+1) - p*B*(4*2*lambda5*lambda7^2 + 2*lambda7^2*delta - ln*delta^2 - 2*lambda5) + p*B*delta + 2*p*B*lambda3 + (4*omega1*omega2 - 2*omega1 - omega2 + 1))*e2 - ln*p*(4*lambda3 + delta + 1)*lambda1*e3)\n",
    "assert(e2*g1 == -p*(2*lambda1 - B*delta)*ln*e0 + p*(-B*(4*lambda3 + delta + 1) + 2*(2*lambda4 + 1))*e1 + 2*C*(2*lambda6+1)*lambda2*e2 - 2*lambda2*(4*lambda3 + delta + 1)*ln*e3)\n",
    "assert(e2*g2 == -2*p*ln*(4*lambda3 + delta + 1)*e0 - 2*p*C*(4*lambda3 + delta + 1)*(2*lambda6+1)*e1 + p*B*(4*lambda3 + delta + 1)*e2 - p*ln*(2*lambda1 - B*delta)*(4*lambda3 + delta + 1)*e3)\n",
    "assert(e2*g3 == -2*p*ln*C*(2*lambda6+1)*e0 + 2*p*(-C^2 + 1)*(2*lambda6+1)^2*e1 + (p*B*C - 2*p*A)*(2*lambda6+1)*e2 - p*ln*B*(4*lambda3 + delta + 1)*e3)\n",
    "assert(e3*g0 == -p*(ln*lc*delta + C)*(2*lambda6+1)*e0 - p*ln*((2*lambda6+1)*C*delta + (4*lambda3 + delta + 1))*e1 + p*lambda1*ln*e2 + (-p*C*(2*lambda1 - B*delta)*(2*lambda6+1) + (-p*ln^2*delta*lambda1 + p*B*(4*2*lambda5*lambda7^2 + 2*lambda7^2*delta - ln*delta^2 - 2*lambda5) + 4*omega1*omega2 - 2*omega1 - omega2 + 1 + 2*p*B*lambda3))*e3)\n",
    "assert(e3*g1 == -p*B*e0 - p*ln*(2*lambda1 - B*delta)*e1 + 2*ln*lambda2*e2 - 2*C*lambda2*(2*lambda6+1)*e3)\n",
    "assert(e3*g2 == -2*p*C*(2*lambda6+1)*e0 - 2*p*ln*(4*lambda3 + delta + 1)*e1 + p*ln*(2*lambda1 - B*delta)*e2 + p*(-2*C*(2*lambda1 - B*delta)*(2*lambda6+1) + (4*lambda3 + delta + 1)*B)*e3)\n",
    "assert(e3*g3 == -2*p*ln^2*e0 - 2*p*ln*(2*lambda6+1)*C*e1 + p*ln*B*e2 - p*(B*C + 2*A)*(2*lambda6+1)*e3)\n",
    "\n",
    "\n",
    "\n",
    "# CASE 2: a+b=n, c=0, a>=0\n",
    "\n",
    "# Define a polynomial ring. Note all variables are integral.\n",
    "R.<p, ln, lb, A, B, C, delta> = PolynomialRing(Rationals())\n",
    "QuatAlg.<i,j,k> = QuaternionAlgebra(-1, -p)\n",
    "\n",
    "# Basis of the lattice using variables above, i.e. replacing \\ell^a with \\ell^n/\\ell^b, and \\ell^c with 1\n",
    "e0 = (1/2) - (C/2)*i + ((B*ln - 2*lb*A*C)/(2*lb))*j - ((2*A*lb + B*C*ln)/(2*lb))*k\n",
    "e1 = (1/2)*i + A*j + ((B*ln)/(2*lb))*k \n",
    "e2 = ln*j\n",
    "e3 = ln*k\n",
    "\n",
    "# Basis of maximal order O\n",
    "g0 = (1/2) + (ln/(2*lb))*j + ((C + delta*lb)/(2))*k\n",
    "g1 = (1/(2*ln))*i + (A/ln)*j + (B/(2*lb))*k\n",
    "g2 = (ln/lb)*j + C*k\n",
    "g3 = lb*k\n",
    "\n",
    "# These are integral by earlier results\n",
    "mu1 = (2*A + B*C + B*delta*lb)/(2*lb)\n",
    "mu2 = (p*ln^2*B^2 + lb^2 + 4*p*A^2*lb^2)/(4*ln^2*lb^2)\n",
    "mu3 = (ln/lb - 1)/2\n",
    "mu4 = (lb + 1)/2\n",
    "omega1 = (p + 1)/4\n",
    "omega2 = (B + 1)/2\n",
    "omega3 = (delta + C)/2\n",
    "\n",
    "# We show the lattice is a right ideal as each e_t * g_s is an integral linear combinations of e_t so lie in the order\n",
    "# Coefficients consist of addition and multiplication of the integer values above (and integral constants) so are all integral\n",
    "assert(e0 == g0 - ln*C*g1 + (omega2-1)*g2 - (mu1 - (omega2-1)*delta)*g3)\n",
    "assert(e1 == ln*g1)\n",
    "assert(e2 == lb*g2 - C*g3)\n",
    "assert(e3 == (2*mu3 + 1)*g3)\n",
    "\n",
    "# We show the lattice is a right ideal as each e_t * g_s is an integral linear combinations of e_t so lie in the order\n",
    "# Coefficients consist of addition and multiplication of the integer values above (and integral constants) so are all integral\n",
    "assert(e0*g0 == (p*(2*mu3 + 1)*B*C*(delta*mu4 + omega3 - delta) - 2*p*mu3*(mu3 + 1)*B - 4*omega2*omega1 + omega2 + 2*omega1 + p*lb*A*delta + p*(2*mu3 + 1)*A*C + p*A*C)*e0 + p*(2*mu3 + 1)*(C^2 + 1)*((B*(delta*mu4 + omega3 - delta) + A))*e1 + (-p*(2*mu3 + 1)*(A*(mu1*2 - B*delta) + mu1*B*C) + 2*p*A*mu3*(mu1*2 - B*delta) + ln*lb*mu2*C*delta + ln*mu2*C^2 - p*A*B*delta + ln*(2*mu3 + 1)*mu2)*e2 + (p*(A*C*(mu1*2 - B*delta) - (2*mu3 + 1)*B*mu1 + A*B*C*delta) + ln*mu2*C - ln*mu2*(2*mu3 + 1)*C + ln*lb*mu2*delta)*e3)\n",
    "assert(e0*g1 == 2*ln*mu2*C*e0 + 2*mu2*ln*(C^2 + 1)*e1 - mu2*((2*mu3 + 1)*B*C + 2*A)*e2 + mu2*(2*A*C - (2*mu3 + 1)*B)*e3)\n",
    "assert(e0*g2 == p*((2*mu3 + 1)*B*C^2 + 2*(2*mu3 + 1)*A*C + 2*A*C - (2*mu3 + 1)^2*B)*e0 + p*(2*mu3 + 1)*(B*C^3 + 2*A*C^2 + B*C + 2*A)*e1 + (2*ln*mu2*C^2 - p*B*C*(2*mu3 + 1)*(mu1*2 - B*delta) - 2*p*A*(mu1*2 - B*delta) + 2*ln*(2*mu3 + 1)*mu2)*e2 + (2*p*A*C*(mu1*2 - B*delta) - p*(2*mu3 + 1)*B*(mu1*2 - B*delta) - 2*ln*(2*mu3 + 1)*mu2*C + 2*ln*mu2*C)*e3)\n",
    "assert(e0*g3 == (p*ln*B*C + 2*p*lb*A)*e0 + (p*ln*B*C^2 + p*ln*B)*e1 + (- p*(2*mu3 + 1)*B^2*C - 2*p*A*B + 2*ln*lb*mu2*C)*e2 + (2*p*A*B*C - p*(2*mu3 + 1)*B^2 + 2*ln*lb*mu2)*e3)\n",
    "assert(e1*g0 == -p*lb*(2*mu3 + 1)*mu1*e0 + (-p*(2*mu3 + 1)*B*C*(delta*mu4 + omega3 - delta) - p*(2*mu3 + 1)^2*B*omega2 + p*lb*A*delta - p*(2*mu3 + 1)*A*C + p*A*C + 2*ln^2*mu2 - 2*p*A^2)*e1 + (-2*ln*mu2*(delta*mu4 + omega3 - delta) + p*B*(2*mu3 + 1)*mu1)*e2 + (-2*p*A*mu1 + ln*(2*mu3 + 1)*mu2)*e3)\n",
    "assert(e1*g1 == -2*ln*mu2*e0 - 2*ln*mu2*C*e1 + (2*mu3 + 1)*mu2*B*e2 - 2*mu2*A*e3)\n",
    "assert(e1*g2 == -p*ln*(mu1*2 - B*delta)*e0 + p*(-(2*mu3 + 1)*B*C^2 - 2*(2*mu3 + 1)*A*C + 2*A*C - (2*mu3 + 1)^2*B)*e1 + (-2*ln*mu2*C + p*(2*mu3 + 1)*(mu1*2 - B*delta)*B)*e2 + (-2*p*(mu1*2 - B*delta)*A + 2*ln*mu2*(2*mu3 + 1))*e3)\n",
    "assert(e1*g3 == -p*ln*B*e0 + (-p*ln*B*C + 2*p*lb*A)*e1 + (-2*ln*lb*mu2 + p*(2*mu3 + 1)*B^2)*e2 - 2*p*A*B*e3)\n",
    "assert(e2*g0 == -p*ln*(2*mu3 + 1)*e0 + p*(ln*lb*delta - ln*(2*mu3 + 1)*C + ln*C)*e1 + (-p*lb*A*delta - p*A*C + 2*ln^2*mu2 - p*(2*mu3 + 1)^2*B*(omega2 - 1) - 2*p*A^2)*e2 - p*(2*mu3 + 1)*lb*mu1*e3)\n",
    "assert(e2*g1 == -2*p*A*e0 + (-2*p*A*C + p*(2*mu3 + 1)*B)*e1 - 2*ln*mu2*e3)\n",
    "assert(e2*g2 == -2*p*ln*(2*mu3 + 1)*e0 + 2*p*ln*C*(1 - (2*mu3 + 1))*e1 + p*(-2*A*C + (2*mu3 + 1)^2*B)*e2 - p*(2*mu3 + 1)*(B*C + 2*A)*e3)\n",
    "assert(e2*g3 == 2*p*ln*lb*e1 - 2*p*lb*A*e2 - p*ln*B*e3)\n",
    "assert(e3*g0 == -p*ln*(lb*delta + C)*e0 + (-p*ln*lb*C*delta - p*ln*C^2 - p*ln*(2*mu3 + 1))*e1 + p*(2*mu3 + 1)*(B*(delta*mu4 + omega3 - delta) + A)*e2 + (-p*lb*A*delta - p*A*C + 2*ln^2*mu2 - 2*p*A^2 - p*(2*mu3 + 1)^2*B*(omega2 - 1))*e3)\n",
    "assert(e3*g1 == -p*(2*mu3 + 1)*B*e0 - p*((2*mu3 + 1)*B*C + 2*A)*e1 + 2*ln*mu2*e2)\n",
    "assert(e3*g2 == -2*p*ln*C*e0 - 2*p*ln*(C^2 + (2*mu3 + 1))*e1 + p*(B*C + 2*A)*(2*mu3 + 1)*e2 + p*(-2*A*C + (2*mu3 + 1)^2*B)*e3)\n",
    "assert(e3*g3 == -2*p*ln*lb*e0 - 2*p*ln*lb*C*e1 + p*ln*B*e2 - 2*p*lb*A*e3)"
   ]
  }
 ],
 "metadata": {
  "kernelspec": {
   "display_name": "SageMath 10.3.beta8",
   "language": "sage",
   "name": "sagemath"
  },
  "language_info": {
   "codemirror_mode": {
    "name": "ipython",
    "version": 3
   },
   "file_extension": ".py",
   "mimetype": "text/x-python",
   "name": "python",
   "nbconvert_exporter": "python",
   "pygments_lexer": "ipython3",
   "version": "3.10.6"
  }
 },
 "nbformat": 4,
 "nbformat_minor": 2
}
